language_formalisation/type_system/bidirectional.v
@@ -5,74 +5,74 @@ Require Import syntax.
 Inductive vsynth : ctx -> val -> vtype -> Type :=
 | SynthUnit Γ : vsynth Γ Unit TyUnit 
 | SynthInt Γ n : vsynth Γ (Int n) TyInt
-| SynthVar Γ id α :
-    get_vtype Γ id = Some α ->
-    vsynth Γ (Var id) α
-| SynthPair Γ v1 v2 α β :
-    vsynth Γ v1 α ->
-    vsynth Γ v2 β ->
-    vsynth Γ (Pair v1 v2) (TyΠ α β)
-| SynthVAnnot Γ v α :
-    vcheck Γ v α ->
-    vsynth Γ (VAnnot v α) α
+| SynthVar Γ id A :
+    get_vtype Γ id = Some A ->
+    vsynth Γ (Var id) A
+| SynthPair Γ v1 v2 A B :
+    vsynth Γ v1 A ->
+    vsynth Γ v2 B ->
+    vsynth Γ (Pair v1 v2) (TyΠ A B)
+| SynthVAnnot Γ v A :
+    vcheck Γ v A ->
+    vsynth Γ (VAnnot v A) A
 with csynth : ctx -> comp -> ctype -> Type :=
-| SynthRet Γ v α : 
-    vsynth Γ v α ->
-    csynth Γ (Ret v) (CTy α SigØ EqsØ)
-| SynthΠMatch Γ v α β x y c ctyC :
-    vsynth Γ v (TyΠ α β) ->
-    csynth (CtxU (CtxU Γ α) β) c ctyC ->
-    csynth Γ (ΠMatch v (x, y) c) ctyC
-| SynthApp Γ v1 v2 α ctyC :
-    vsynth Γ v1 (TyFun α ctyC) ->
-    vcheck Γ v2 α ->
-    csynth Γ (App v1 v2) ctyC
-| SynthHandle Γ v c ctyC ctyD :
-    vsynth Γ v (TyHandler ctyC ctyD) ->
-    ccheck Γ c ctyC ->
-    csynth Γ (Handle v c) ctyD
-| SynthCAnnot Γ c ctyC :
-    ccheck Γ c ctyC ->
-    csynth Γ (CAnnot c ctyC) ctyC
+| SynthRet Γ v A : 
+    vsynth Γ v A ->
+    csynth Γ (Ret v) (CTy A SigØ EqsØ)
+| SynthΠMatch Γ v A B x y c C :
+    vsynth Γ v (TyΠ A B) ->
+    csynth (CtxU (CtxU Γ A) B) c C ->
+    csynth Γ (ΠMatch v (x, y) c) C
+| SynthApp Γ v1 v2 A C :
+    vsynth Γ v1 (TyFun A C) ->
+    vcheck Γ v2 A ->
+    csynth Γ (App v1 v2) C
+| SynthHandle Γ v c C D :
+    vsynth Γ v (TyHandler C D) ->
+    ccheck Γ c C ->
+    csynth Γ (Handle v c) D
+| SynthCAnnot Γ c C :
+    ccheck Γ c C ->
+    csynth Γ (CAnnot c C) C
 | SynthLetRec Γ f x A C c1 c2 D:
     ccheck (CtxU (CtxU Γ A) (TyFun A C)) c1 C ->
     csynth (CtxU Γ (TyFun A C)) c2 D ->
     csynth Γ (LetRec f x (TyFun A C) c1 c2) D
 (* with hsynth : ctx -> hcases -> sig -> ctype -> Type := *)
 with vcheck : ctx -> val -> vtype -> Type :=
-| CheckVBySynth Γ v α : vsynth Γ v α -> vcheck Γ v α
-| CheckInl Γ v α β :
-    vcheck Γ v α ->
-    vcheck Γ (Inl v) (TyΣ α β)
-| CheckInr Γ v α β :
-    vcheck Γ v β ->
-    vcheck Γ (Inr v) (TyΣ α β)
-| CheckFun Γ x c α C :
-    ccheck (CtxU Γ α) c C ->
-    vcheck Γ (Fun x c) (TyFun α C)
-| CheckHandler Γ x c_ret h α sig eqs D :
-    ccheck (CtxU Γ α) c_ret D ->
+| CheckVBySynth Γ v A : vsynth Γ v A -> vcheck Γ v A
+| CheckInl Γ v A B :
+    vcheck Γ v A ->
+    vcheck Γ (Inl v) (TyΣ A B)
+| CheckInr Γ v A B :
+    vcheck Γ v B ->
+    vcheck Γ (Inr v) (TyΣ A B)
+| CheckFun Γ x c A C :
+    ccheck (CtxU Γ A) c C ->
+    vcheck Γ (Fun x c) (TyFun A C)
+| CheckHandler Γ x c_ret h A sig eqs D :
+    ccheck (CtxU Γ A) c_ret D ->
     hcheck Γ h sig D ->
-    vcheck Γ (Handler x c_ret h) (TyHandler (CTy α sig eqs) D)
+    vcheck Γ (Handler x c_ret h) (TyHandler (CTy A sig eqs) D)
 with ccheck : ctx -> comp -> ctype -> Type :=
 | CheckCBySynth Γ c C C' : csynth Γ c C' -> C = C' -> ccheck Γ c C
-| CheckΣMatch Γ v α β xl cl xr cr C :
-    vsynth Γ v (TyΣ α β) ->
-    ccheck (CtxU Γ α) cl C ->
-    ccheck (CtxU Γ β) cr C ->
+| CheckΣMatch Γ v A B xl cl xr cr C :
+    vsynth Γ v (TyΣ A B) ->
+    ccheck (CtxU Γ A) cl C ->
+    ccheck (CtxU Γ B) cr C ->
     ccheck Γ (ΣMatch v xl cl xr cr) C
-| CheckOp Γ op_id v y c α_op β_op α Σ eqs :
-    get_op_type Σ op_id = Some (α_op, β_op) ->
-    vcheck Γ v α_op ->
-    ccheck (CtxU Γ β_op) c (CTy α Σ eqs) ->
-    ccheck Γ (Op op_id v y c) (CTy α Σ eqs)
+| CheckOp Γ op_id v y c A_op B_op A Σ eqs :
+    get_op_type Σ op_id = Some (A_op, B_op) ->
+    vcheck Γ v A_op ->
+    ccheck (CtxU Γ B_op) c (CTy A Σ eqs) ->
+    ccheck Γ (Op op_id v y c) (CTy A Σ eqs)
 with hcheck : ctx -> hcases -> sig -> ctype -> Type :=
 | CheckCasesØ Γ D : hcheck Γ CasesØ SigØ D
-| CheckCasesU Γ h op_id x k c_op α_op β_op Σ D :
+| CheckCasesU Γ h op_id x k c_op A_op B_op Σ D :
     find_op_case h op_id = None ->
     hcheck Γ h Σ D ->
-    ccheck (CtxU (CtxU Γ (TyFun β_op D)) α_op) c_op D ->
+    ccheck (CtxU (CtxU Γ (TyFun B_op D)) A_op) c_op D ->
     hcheck 
       Γ (CasesU h op_id x k c_op)
-      (SigU Σ op_id α_op β_op) D
+      (SigU Σ op_id A_op B_op) D
 .
