language_formalisation/type_system/declarational.v
@@ -1,0 +1,137 @@
+Add LoadPath "C:\Users\Ziga\Documents\Ziga_podatki\PHD\language_formalisation\syntax".
+Add LoadPath "C:\Users\Ziga\Documents\Ziga_podatki\PHD\language_formalisation\type_system".
+(* Add LoadPath "E:\Ziga_Podatki\faks\PHD\language_formalisation\syntax". *)
+Require Import syntax bidirectional.
+
+Inductive has_vtype : ctx -> val -> vtype -> Type :=
+| TypeUnit Γ : has_vtype Γ Unit TyUnit 
+| TypeInt Γ n : has_vtype Γ (Int n) TyInt
+| TypeVar Γ id A :
+    get_vtype Γ id = Some A ->
+    has_vtype Γ (Var id) A
+| TypePair Γ v1 v2 A B :
+    has_vtype Γ v1 A ->
+    has_vtype Γ v2 B ->
+    has_vtype Γ (Pair v1 v2) (TyΠ A B)
+| TypeVAnnot Γ v A :
+    has_vtype Γ v A ->
+    has_vtype Γ (VAnnot v A) A
+| TypeInl Γ v A B :
+    has_vtype Γ v A ->
+    has_vtype Γ (Inl v) (TyΣ A B)
+| TypeInr Γ v A B :
+    has_vtype Γ v B ->
+    has_vtype Γ (Inr v) (TyΣ A B)
+| TypeFun Γ x c A C :
+    has_ctype (CtxU Γ A) c C ->
+    has_vtype Γ (Fun x c) (TyFun A C)
+| TypeHandler Γ x c_ret h A sig eqs D :
+    has_ctype (CtxU Γ A) c_ret D ->
+    has_htype Γ h sig D ->
+    has_vtype Γ (Handler x c_ret h) (TyHandler (CTy A sig eqs) D)
+with has_ctype : ctx -> comp -> ctype -> Type :=
+| TypeRet Γ v A : 
+    has_vtype Γ v A ->
+    has_ctype Γ (Ret v) (CTy A SigØ EqsØ)
+| TypeΠMatch Γ v A B x y c C :
+    has_vtype Γ v (TyΠ A B) ->
+    has_ctype (CtxU (CtxU Γ A) B) c C ->
+    has_ctype Γ (ΠMatch v (x, y) c) C
+| TypeApp Γ v1 v2 A C :
+    has_vtype Γ v1 (TyFun A C) ->
+    has_vtype Γ v2 A ->
+    has_ctype Γ (App v1 v2) C
+| TypeHandle Γ v c C D :
+    has_vtype Γ v (TyHandler C D) ->
+    has_ctype Γ c C ->
+    has_ctype Γ (Handle v c) D
+| TypeCAnnot Γ c C :
+    has_ctype Γ c C ->
+    has_ctype Γ (CAnnot c C) C
+| TypeLetRec Γ f x A C c1 c2 D:
+    has_ctype (CtxU (CtxU Γ A) (TyFun A C)) c1 C ->
+    has_ctype (CtxU Γ (TyFun A C)) c2 D ->
+    has_ctype Γ (LetRec f x (TyFun A C) c1 c2) D
+| TypeΣMatch Γ v A B xl cl xr cr C :
+    has_vtype Γ v (TyΣ A B) ->
+    has_ctype (CtxU Γ A) cl C ->
+    has_ctype (CtxU Γ B) cr C ->
+    has_ctype Γ (ΣMatch v xl cl xr cr) C
+| TypeOp Γ op_id v y c A_op B_op A Σ eqs :
+    get_op_type Σ op_id = Some (A_op, B_op) ->
+    has_vtype Γ v A_op ->
+    has_ctype (CtxU Γ B_op) c (CTy A Σ eqs) ->
+    has_ctype Γ (Op op_id v y c) (CTy A Σ eqs)
+with has_htype : ctx -> hcases -> sig -> ctype -> Type :=
+| TypeCasesØ Γ D : has_htype Γ CasesØ SigØ D
+| TypeCasesU Γ h op_id x k c_op A_op B_op Σ D :
+    find_op_case h op_id = None ->
+    has_htype Γ h Σ D ->
+    has_ctype (CtxU (CtxU Γ (TyFun B_op D)) A_op) c_op D ->
+    has_htype 
+      Γ (CasesU h op_id x k c_op)
+      (SigU Σ op_id A_op B_op) D
+.
+
+Ltac inv H := inversion H; clear H; subst.
+
+
+Fixpoint vcheck_has_vtype Γ v A {struct v}:
+  vcheck Γ v A -> has_vtype Γ v A
+with vsynth_has_vtype Γ v A {struct v}:
+  vsynth Γ v A -> has_vtype Γ v A
+with ccheck_has_ctype Γ c C {struct c}:
+  ccheck Γ c C -> has_ctype Γ c C
+with csynth_has_ctype Γ c C {struct c}:
+  csynth Γ c C -> has_ctype Γ c C
+with hcheck_has_htype Γ h Σ D {struct h}:
+  hcheck Γ h Σ D -> has_htype Γ h Σ D.
+Proof.
+{
+clear vcheck_has_vtype.
+revert Γ A. induction v; intros Γ A orig; inv orig; try inv H.
++ apply TypeVar. assumption.
++ apply TypeUnit.
++ apply TypeInt.
++ apply TypeInl. apply IHv. assumption.
++ apply TypeInr. apply IHv. assumption.
++ apply TypePair; auto.
++ apply TypeFun. auto.
++ apply TypeHandler; auto.
++ apply TypeVAnnot; auto.
+}{
+clear vsynth_has_vtype.
+revert Γ A. induction v; intros Γ A orig; inv orig.
++ apply TypeVar. assumption.
++ apply TypeUnit.
++ apply TypeInt.
++ apply TypePair; auto.
++ apply TypeVAnnot. auto.
+}{
+clear ccheck_has_ctype.
+revert Γ C. induction c; intros Γ C orig; inv orig; try inv H.
++ apply TypeRet. auto.
++ eapply TypeΠMatch. apply vsynth_has_vtype; exact H5.
+  apply csynth_has_ctype. assumption.
++ eapply TypeΣMatch. apply vsynth_has_vtype; exact H6. auto. auto.
++ eapply TypeApp. apply vsynth_has_vtype. exact H3. auto.
++ eapply TypeOp; try exact H5 || auto.
++ apply TypeLetRec; auto.
++ eapply TypeHandle. apply vsynth_has_vtype. exact H3. auto.
++ apply TypeCAnnot. auto. 
+}{
+clear csynth_has_ctype.
+revert Γ C. induction c; intros Γ C orig; inv orig.
++ apply TypeRet. auto.
++ eapply TypeΠMatch. apply vsynth_has_vtype; exact H4. auto.
++ eapply TypeApp. apply vsynth_has_vtype; exact H2. auto.
++ apply TypeLetRec. auto. apply IHc2. assumption.
++ eapply TypeHandle. apply vsynth_has_vtype; exact H2. auto.
++ eapply TypeCAnnot. auto.
+}{
+clear hcheck_has_htype.
+revert Γ Σ D. induction h; intros Γ Σ D orig; inv orig.
++ apply TypeCasesØ.
++ apply TypeCasesU; auto.
+}
+Qed.
