language_formalisation/type_system/lemmas.v
@@ -9,46 +9,46 @@ Require Export syntax bidirectional substitution
 Ltac inv H := inversion H; clear H; subst.
 
 Lemma v_subs_checksafe
-  (Γ:ctx) (v:val) (A:vtype) (i:nat) (v_s:val) (α:vtype) :
-  vcheck Γ v A -> get_vtype_i Γ i = Some α ->
-  vcheck Γ v_s α ->
+  (Γ:ctx) (v:val) (A:vtype) (i:nat) (v_s:val) (A:vtype) :
+  vcheck Γ v A -> get_vtype_i Γ i = Some A ->
+  vcheck Γ v_s A ->
   vcheck Γ (Sub.v_sub v (i, v_s)) A
 Lemma v_subs_synthsafe
-  (Γ:ctx) (v:val) (A:vtype) (i:nat) (v_s:val) (α:vtype) :
-  vsynth Γ v A -> get_vtype_i Γ i = Some α ->
-  vcheck Γ v_s α ->
+  (Γ:ctx) (v:val) (A:vtype) (i:nat) (v_s:val) (A:vtype) :
+  vsynth Γ v A -> get_vtype_i Γ i = Some A ->
+  vcheck Γ v_s A ->
   vsynth Γ (Sub.v_sub v (i, v_s)) A
 
 
 (* 
 Lemma vcheck_sub_lemma 
-  (Γ:ctx) (v:val) (A:vtype) (v_s:val) (α:vtype) :
-  vcheck (CtxU Γ α) v A ->
-  vcheck Γ v_s α ->
+  (Γ:ctx) (v:val) (A:vtype) (v_s:val) (A:vtype) :
+  vcheck (CtxU Γ A) v A ->
+  vcheck Γ v_s A ->
   vcheck Γ (vsub_out v v_s) A
 
 with vsynth_sub_lemma 
-  (Γ:ctx) (v:val) (A:vtype) (v_s:val) (α:vtype) :
-  vsynth (CtxU Γ α) v A ->
-  vcheck Γ v_s α ->
+  (Γ:ctx) (v:val) (A:vtype) (v_s:val) (A:vtype) :
+  vsynth (CtxU Γ A) v A ->
+  vcheck Γ v_s A ->
   vsynth Γ (vsub_out v v_s) A
 
 with ccheck_sub_lemma 
-  (Γ:ctx) (c:comp) (C:ctype) (v_s:val) (α:vtype) :
-  ccheck (CtxU Γ α) c C ->
-  vcheck Γ v_s α ->
+  (Γ:ctx) (c:comp) (C:ctype) (v_s:val) (A:vtype) :
+  ccheck (CtxU Γ A) c C ->
+  vcheck Γ v_s A ->
   ccheck Γ (csub_out c v_s) C
 
 with csynth_sub_lemma 
-  (Γ:ctx) (c:comp) (C:ctype) (v_s:val) (α:vtype) :
-  csynth (CtxU Γ α) c C ->
-  vcheck Γ v_s α ->
+  (Γ:ctx) (c:comp) (C:ctype) (v_s:val) (A:vtype) :
+  csynth (CtxU Γ A) c C ->
+  vcheck Γ v_s A ->
   csynth Γ (csub_out c v_s) C
 
 with hcheck_sub_lemma 
-  (Γ:ctx) (h:hcases) (Σ:sig) (D:ctype) (v_s:val) (α:vtype) :
-  hcheck (CtxU Γ α) h Σ D ->
-  vcheck Γ v_s α ->
+  (Γ:ctx) (h:hcases) (Σ:sig) (D:ctype) (v_s:val) (A:vtype) :
+  hcheck (CtxU Γ A) h Σ D ->
+  vcheck Γ v_s A ->
   hcheck Γ (hsub_out h v_s) Σ D.
 
 Proof. *)
