language_formalisation/type_system/type_aux_lemmas.v
@@ -12,8 +12,8 @@ Require Export syntax syntax_lemmas bidirectional substitution Omega Logic.
 Ltac inv H := inversion H; clear H; subst.
 
 
-Lemma extend_get_proof Γ α i αi:
-  get_vtype_i Γ i = Some αi-> get_vtype_i (CtxU Γ α) (i + 1) = Some αi.
+Lemma extend_get_proof Γ A i Ai:
+  get_vtype_i Γ i = Some Ai-> get_vtype_i (CtxU Γ A) (i + 1) = Some Ai.
 Proof.
 assert (i + 1 = S i) by omega.
 induction Γ; rewrite H; auto.
@@ -21,45 +21,45 @@ Qed.
 
 (* Switch lemmas *)
 Fixpoint v_switch_checksafe
-  (Γ:ctx) i (αi:vtype) j (αj:vtype) (v:val) (A:vtype)
-  (p_i : get_vtype_i Γ i = Some αi) (p_j : get_vtype_i Γ j = Some αj) 
+  (Γ:ctx) i (Ai:vtype) j (Aj:vtype) (v:val) (A:vtype)
+  (p_i : get_vtype_i Γ i = Some Ai) (p_j : get_vtype_i Γ j = Some Aj) 
   {struct v} :
   vcheck Γ v A ->
-  vcheck (ctx_switch_vars Γ i j αi αj p_i p_j) (v_switch_vars v i j) A
+  vcheck (ctx_switch_vars Γ i j Ai Aj p_i p_j) (v_switch_vars v i j) A
 
 with v_switch_synthsafe
-  (Γ:ctx) i (αi:vtype) j (αj:vtype) (v:val) (A:vtype)
-  (p_i : get_vtype_i Γ i = Some αi) (p_j : get_vtype_i Γ j = Some αj)
+  (Γ:ctx) i (Ai:vtype) j (Aj:vtype) (v:val) (A:vtype)
+  (p_i : get_vtype_i Γ i = Some Ai) (p_j : get_vtype_i Γ j = Some Aj)
   {struct v}:
   vsynth Γ v A ->
-  vsynth (ctx_switch_vars Γ i j αi αj p_i p_j) (v_switch_vars v i j) A
+  vsynth (ctx_switch_vars Γ i j Ai Aj p_i p_j) (v_switch_vars v i j) A
 
 with c_switch_checksafe 
-  (Γ:ctx) i (αi:vtype) j (αj:vtype) (c:comp) (C:ctype)
-  (p_i : get_vtype_i Γ i = Some αi) (p_j : get_vtype_i Γ j = Some αj)
+  (Γ:ctx) i (Ai:vtype) j (Aj:vtype) (c:comp) (C:ctype)
+  (p_i : get_vtype_i Γ i = Some Ai) (p_j : get_vtype_i Γ j = Some Aj)
   {struct c}:
   ccheck Γ c C -> 
-  ccheck (ctx_switch_vars Γ i j αi αj p_i p_j) (c_switch_vars c i j) C
+  ccheck (ctx_switch_vars Γ i j Ai Aj p_i p_j) (c_switch_vars c i j) C
 
 with c_switch_synthsafe 
-  (Γ:ctx) i (αi:vtype) j (αj:vtype) (c:comp) (C:ctype)
-  (p_i : get_vtype_i Γ i = Some αi) (p_j : get_vtype_i Γ j = Some αj)
+  (Γ:ctx) i (Ai:vtype) j (Aj:vtype) (c:comp) (C:ctype)
+  (p_i : get_vtype_i Γ i = Some Ai) (p_j : get_vtype_i Γ j = Some Aj)
   {struct c}:
   csynth Γ c C -> 
-  csynth (ctx_switch_vars Γ i j αi αj p_i p_j) (c_switch_vars c i j) C
+  csynth (ctx_switch_vars Γ i j Ai Aj p_i p_j) (c_switch_vars c i j) C
 
 with h_switch_checksafe
-  (Γ:ctx) i (αi:vtype) j (αj:vtype) (h:hcases) (Σ:sig) (D:ctype)
-  (p_i : get_vtype_i Γ i = Some αi) (p_j : get_vtype_i Γ j = Some αj)
+  (Γ:ctx) i (Ai:vtype) j (Aj:vtype) (h:hcases) (Σ:sig) (D:ctype)
+  (p_i : get_vtype_i Γ i = Some Ai) (p_j : get_vtype_i Γ j = Some Aj)
   {struct h}:
   hcheck Γ h Σ D ->
-  hcheck (ctx_switch_vars Γ i j αi αj p_i p_j) (h_switch_vars h i j) Σ D.
+  hcheck (ctx_switch_vars Γ i j Ai Aj p_i p_j) (h_switch_vars h i j) Σ D.
 Proof.
 {
 clear v_switch_checksafe.
 clear c_switch_synthsafe.
-revert Γ i j αi αj A p_i p_j; induction v;
-intros Γ i j αi αj A p_i p_j orig.
+revert Γ i j Ai Aj A p_i p_j; induction v;
+intros Γ i j Ai Aj A p_i p_j orig.
 
 all: inv orig; try inv H.
 { (* relevant case *)
@@ -86,17 +86,17 @@ all: inv orig; try inv H.
 + apply CheckInl. apply IHv. assumption.
 + apply CheckInr. apply IHv. assumption.
 + apply CheckVBySynth. apply SynthPair.
-  apply (v_switch_synthsafe _ i αi j αj _ _ p_i p_j) in H3. assumption.
-  apply (v_switch_synthsafe _ i αi j αj _ _ p_i p_j) in H5. assumption.
+  apply (v_switch_synthsafe _ i Ai j Aj _ _ p_i p_j) in H3. assumption.
+  apply (v_switch_synthsafe _ i Ai j Aj _ _ p_i p_j) in H5. assumption.
 + apply CheckFun.
-  apply (extend_get_proof _ α) in p_i as pp_i.
-  apply (extend_get_proof _ α) in p_j as pp_j.
-  rewrite (ctx_switch_extend1 Γ α i j αi αj p_i p_j pp_i pp_j).
+  apply (extend_get_proof _ A0) in p_i as pp_i.
+  apply (extend_get_proof _ A0) in p_j as pp_j.
+  rewrite (ctx_switch_extend1 Γ A0 i j Ai Aj p_i p_j pp_i pp_j).
   apply c_switch_checksafe. assumption.
 + apply CheckHandler.
-  * apply (extend_get_proof _ α) in p_i as pp_i.
-    apply (extend_get_proof _ α) in p_j as pp_j.
-    rewrite (ctx_switch_extend1 Γ α i j αi αj p_i p_j pp_i pp_j).
+  * apply (extend_get_proof _ A0) in p_i as pp_i.
+    apply (extend_get_proof _ A0) in p_j as pp_j.
+    rewrite (ctx_switch_extend1 Γ A0 i j Ai Aj p_i p_j pp_i pp_j).
     apply c_switch_checksafe. assumption.
   * apply h_switch_checksafe. assumption.
 + apply CheckVBySynth. apply SynthVAnnot. apply IHv. assumption.
@@ -105,8 +105,8 @@ all: inv orig; try inv H.
 clear v_switch_synthsafe.
 clear c_switch_synthsafe.
 clear h_switch_checksafe.
-revert Γ i j αi αj A p_i p_j; induction v;
-intros Γ i j αi αj A p_i p_j orig; inv orig; try inv H; simpl.
+revert Γ i j Ai Aj A p_i p_j; induction v;
+intros Γ i j Ai Aj A p_i p_j orig; inv orig; try inv H; simpl.
 { (* relevant case *)
   destruct v as (name, num).
   remember (num =? i) as cmpi.
@@ -133,40 +133,40 @@ intros Γ i j αi αj A p_i p_j orig; inv orig; try inv H; simpl.
 {
 clear c_switch_checksafe.
 clear h_switch_checksafe.
-revert Γ i j αi αj C p_i p_j; induction c;
-intros Γ i j αi αj C p_i p_j orig; inv orig; try inv H.
-+ remember (CTy α SigØ EqsØ) as C.
+revert Γ i j Ai Aj C p_i p_j; induction c;
+intros Γ i j Ai Aj C p_i p_j orig; inv orig; try inv H.
++ remember (CTy A SigØ EqsØ) as C.
   apply (CheckCBySynth _ _ C C); try reflexivity.
   rewrite HeqC. apply SynthRet.
   apply v_switch_synthsafe. assumption.
 + apply (CheckCBySynth _ _ C' C'); try reflexivity.
-  apply (SynthΠMatch _ _ α β).
+  apply (SynthΠMatch _ _ A B).
   apply v_switch_synthsafe. assumption.
   clear v_switch_checksafe.
-  apply (extend_get_proof _ α) in p_i as pp_i.
-  apply (extend_get_proof _ α) in p_j as pp_j.
-  apply (extend_get_proof _ β) in pp_i.
-  apply (extend_get_proof _ β) in pp_j.
+  apply (extend_get_proof _ A) in p_i as pp_i.
+  apply (extend_get_proof _ A) in p_j as pp_j.
+  apply (extend_get_proof _ B) in pp_i.
+  apply (extend_get_proof _ B) in pp_j.
   assert (i+1+1=i+2) by omega. rewrite H in pp_i.
   assert (j+1+1=j+2) by omega. rewrite H0 in pp_j.
   rewrite (ctx_switch_extend2 _ _ _ _ _ _ _ p_i p_j pp_i pp_j).
   apply c_switch_synthsafe; assumption.
-+ apply (CheckΣMatch _ _ α β); try apply v_switch_synthsafe; auto.
-  - apply (extend_get_proof _ α) in p_i as pp_i;
-    apply (extend_get_proof _ α) in p_j as pp_j.
-    rewrite (ctx_switch_extend1 Γ α i j αi αj p_i p_j pp_i pp_j).
++ apply (CheckΣMatch _ _ A B); try apply v_switch_synthsafe; auto.
+  - apply (extend_get_proof _ A) in p_i as pp_i;
+    apply (extend_get_proof _ A) in p_j as pp_j.
+    rewrite (ctx_switch_extend1 Γ A i j Ai Aj p_i p_j pp_i pp_j).
     apply IHc1. assumption.
-  - apply (extend_get_proof _ β) in p_i as pp_i;
-    apply (extend_get_proof _ β) in p_j as pp_j.
-    rewrite (ctx_switch_extend1 Γ β i j αi αj p_i p_j pp_i pp_j).
+  - apply (extend_get_proof _ B) in p_i as pp_i;
+    apply (extend_get_proof _ B) in p_j as pp_j.
+    rewrite (ctx_switch_extend1 Γ B i j Ai Aj p_i p_j pp_i pp_j).
     apply IHc2. assumption.
 + apply (CheckCBySynth _ _ C' C'); try reflexivity.
-  apply (SynthApp _ _ _ α C'). apply v_switch_synthsafe; assumption.
+  apply (SynthApp _ _ _ A C'). apply v_switch_synthsafe; assumption.
   apply v_switch_checksafe. assumption.
-+ simpl. apply (CheckOp _ _ _ _ _ α_op β_op α Σ eqs); auto.
-  apply (extend_get_proof _ β_op) in p_i as pp_i.
-  apply (extend_get_proof _ β_op) in p_j as pp_j.
-  rewrite (ctx_switch_extend1 Γ β_op i j αi αj p_i p_j pp_i pp_j).
++ simpl. apply (CheckOp _ _ _ _ _ A_op B_op A Σ eqs); auto.
+  apply (extend_get_proof _ B_op) in p_i as pp_i.
+  apply (extend_get_proof _ B_op) in p_j as pp_j.
+  rewrite (ctx_switch_extend1 Γ B_op i j Ai Aj p_i p_j pp_i pp_j).
   apply IHc. assumption.
 + apply (CheckCBySynth _ _ C' C'); try reflexivity.
   apply SynthLetRec.
@@ -183,7 +183,7 @@ intros Γ i j αi αj C p_i p_j orig; inv orig; try inv H.
     rewrite (ctx_switch_extend1 _ _ _ _ _ _  p_i p_j pp_i pp_j).
     apply c_switch_synthsafe. assumption.
 + apply (CheckCBySynth _ _ C' C'); try reflexivity.
-  apply (SynthHandle _ _ _ ctyC).
+  apply (SynthHandle _ _ _ C).
   - apply v_switch_synthsafe. assumption.
   - apply IHc. assumption.
 + apply (CheckCBySynth _ _ C' C'); try reflexivity.
@@ -192,21 +192,21 @@ intros Γ i j αi αj C p_i p_j orig; inv orig; try inv H.
 {
 clear c_switch_synthsafe.
 clear h_switch_checksafe.
-revert Γ i j αi αj C p_i p_j; induction c;
-intros Γ i j αi αj C p_i p_j orig; inv orig; try inv H; simpl.
+revert Γ i j Ai Aj C p_i p_j; induction c;
+intros Γ i j Ai Aj C p_i p_j orig; inv orig; try inv H; simpl.
 + apply SynthRet. apply v_switch_synthsafe. assumption.
-+ apply (SynthΠMatch _ _ α β).
++ apply (SynthΠMatch _ _ A B).
   apply v_switch_synthsafe. assumption.
   clear v_switch_checksafe.
-  apply (extend_get_proof _ α) in p_i as pp_i.
-  apply (extend_get_proof _ α) in p_j as pp_j.
-  apply (extend_get_proof _ β) in pp_i.
-  apply (extend_get_proof _ β) in pp_j.
+  apply (extend_get_proof _ A) in p_i as pp_i.
+  apply (extend_get_proof _ A) in p_j as pp_j.
+  apply (extend_get_proof _ B) in pp_i.
+  apply (extend_get_proof _ B) in pp_j.
   assert (i+1+1=i+2) by omega. rewrite H in pp_i.
   assert (j+1+1=j+2) by omega. rewrite H0 in pp_j.
   rewrite (ctx_switch_extend2 _ _ _ _ _ _ _ p_i p_j pp_i pp_j).
   apply IHc. assumption.
-+ apply (SynthApp _ _ _ α C).
++ apply (SynthApp _ _ _ A C).
   - apply v_switch_synthsafe. assumption.
   - apply v_switch_checksafe. assumption.
 + apply (SynthLetRec).
@@ -222,7 +222,7 @@ intros Γ i j αi αj C p_i p_j orig; inv orig; try inv H; simpl.
     apply (extend_get_proof _ (TyFun A C0)) in p_j as pp_j.
     rewrite (ctx_switch_extend1 _ _ _ _ _ _  p_i p_j pp_i pp_j).
     apply IHc2. assumption.
-+ apply (SynthHandle _ _ _ ctyC C).
++ apply (SynthHandle _ _ _ C0 C).
   - apply v_switch_synthsafe. assumption.
   - apply c_switch_checksafe. assumption.
 + apply SynthCAnnot. apply c_switch_checksafe. assumption.
@@ -230,16 +230,16 @@ intros Γ i j αi αj C p_i p_j orig; inv orig; try inv H; simpl.
 {
 clear c_switch_synthsafe.
 clear h_switch_checksafe.
-revert Γ i j αi αj Σ D p_i p_j; induction h;
-intros Γ i j αi αj Σ D p_i p_j orig; inv orig; try inv H; simpl.
+revert Γ i j Ai Aj Σ D p_i p_j; induction h;
+intros Γ i j Ai Aj Σ D p_i p_j orig; inv orig; try inv H; simpl.
 apply CheckCasesØ.
 apply CheckCasesU.
 + apply find_op_None_switch. assumption.
 + apply IHh. assumption.
-+ apply (extend_get_proof _ (TyFun β_op D)) in p_i as pp_i.
-  apply (extend_get_proof _ (TyFun β_op D)) in p_j as pp_j.
-  apply (extend_get_proof _ α_op) in pp_i.
-  apply (extend_get_proof _ α_op) in pp_j.
++ apply (extend_get_proof _ (TyFun B_op D)) in p_i as pp_i.
+  apply (extend_get_proof _ (TyFun B_op D)) in p_j as pp_j.
+  apply (extend_get_proof _ A_op) in pp_i.
+  apply (extend_get_proof _ A_op) in pp_j.
   assert (i+1+1=i+2) by omega. rewrite H in pp_i.
   assert (j+1+1=j+2) by omega. rewrite H0 in pp_j.
   rewrite (ctx_switch_extend2 _ _ _ _ _ _ _ p_i p_j pp_i pp_j).
@@ -249,41 +249,41 @@ Qed.
 
 (* Switch lemmas *)
 Fixpoint v_switch10_checksafe
-  (Γ:ctx) (α1:vtype) (α0:vtype) (v:val) (A:vtype)
+  (Γ:ctx) (A1:vtype) (A0:vtype) (v:val) (A:vtype)
   {struct v} :
-  vcheck (CtxU (CtxU Γ α1) α0) v A ->
-  vcheck (CtxU (CtxU Γ α0) α1) (v_switch_vars v 1 0) A
+  vcheck (CtxU (CtxU Γ A1) A0) v A ->
+  vcheck (CtxU (CtxU Γ A0) A1) (v_switch_vars v 1 0) A
 
 with v_switch10_synthsafe
-  (Γ:ctx) (α1:vtype) (α0:vtype) (v:val) (A:vtype)
+  (Γ:ctx) (A1:vtype) (A0:vtype) (v:val) (A:vtype)
   {struct v}:
-  vsynth (CtxU (CtxU Γ α1) α0) v A ->
-  vsynth (CtxU (CtxU Γ α0) α1) (v_switch_vars v 1 0) A
+  vsynth (CtxU (CtxU Γ A1) A0) v A ->
+  vsynth (CtxU (CtxU Γ A0) A1) (v_switch_vars v 1 0) A
 
 with c_switch10_checksafe 
-  (Γ:ctx) (α1:vtype) (α0:vtype) (c:comp) (C:ctype)
+  (Γ:ctx) (A1:vtype) (A0:vtype) (c:comp) (C:ctype)
   {struct c}:
-  ccheck (CtxU (CtxU Γ α1) α0) c C -> 
-  ccheck (CtxU (CtxU Γ α0) α1) (c_switch_vars c 1 0) C
+  ccheck (CtxU (CtxU Γ A1) A0) c C -> 
+  ccheck (CtxU (CtxU Γ A0) A1) (c_switch_vars c 1 0) C
 
 with c_switch10_synthsafe 
-  (Γ:ctx) (α1:vtype) (α0:vtype) (c:comp) (C:ctype)
+  (Γ:ctx) (A1:vtype) (A0:vtype) (c:comp) (C:ctype)
   {struct c}:
-  csynth (CtxU (CtxU Γ α1) α0) c C -> 
-  csynth (CtxU (CtxU Γ α0) α1) (c_switch_vars c 1 0) C
+  csynth (CtxU (CtxU Γ A1) A0) c C -> 
+  csynth (CtxU (CtxU Γ A0) A1) (c_switch_vars c 1 0) C
 
 with h_switch10_checksafe
-  (Γ:ctx) (α1:vtype) (α0:vtype) (h:hcases) (Σ:sig) (D:ctype)
+  (Γ:ctx) (A1:vtype) (A0:vtype) (h:hcases) (Σ:sig) (D:ctype)
   {struct h}:
-  hcheck (CtxU (CtxU Γ α1) α0) h Σ D ->
-  hcheck (CtxU (CtxU Γ α0) α1) (h_switch_vars h 1 0) Σ D.
+  hcheck (CtxU (CtxU Γ A1) A0) h Σ D ->
+  hcheck (CtxU (CtxU Γ A0) A1) (h_switch_vars h 1 0) Σ D.
 Proof.
-all: intro orig; remember (CtxU (CtxU Γ α1) α0) as Γ'.
-all: assert (get_vtype_i Γ' 1 = Some α1) as p_1.
+all: intro orig; remember (CtxU (CtxU Γ A1) A0) as Γ'.
+all: assert (get_vtype_i Γ' 1 = Some A1) as p_1.
 all: try (rewrite HeqΓ'; simpl; f_equal).
-all: assert (get_vtype_i Γ' 0 = Some α0) as p_0.
+all: assert (get_vtype_i Γ' 0 = Some A0) as p_0.
 all: try (rewrite HeqΓ'; simpl; f_equal).
-all: assert (ctx_switch_vars Γ' 1 0 α1 α0 p_1 p_0 = CtxU (CtxU Γ α0) α1).
+all: assert (ctx_switch_vars Γ' 1 0 A1 A0 p_1 p_0 = CtxU (CtxU Γ A0) A1).
 all: try (unfold ctx_switch_vars; rewrite HeqΓ'; simpl; f_equal).
 all: rewrite <-H.
 + apply v_switch_checksafe. assumption.
@@ -299,49 +299,49 @@ Definition h_switch210_vars h := (h_switch_vars (h_switch_vars h 1 0) 2 1).
 
 (* Switch lemmas *)
 Fixpoint v_switch210_checksafe
-  (Γ:ctx) (α2 : vtype) (α1:vtype) (α0:vtype) (v:val) (A:vtype)
+  (Γ:ctx) (A2 : vtype) (A1:vtype) (A0:vtype) (v:val) (A:vtype)
   {struct v} :
-  vcheck (CtxU (CtxU (CtxU Γ α2) α1) α0) v A ->
-  vcheck (CtxU (CtxU (CtxU Γ α0) α2) α1) (v_switch210_vars v) A
+  vcheck (CtxU (CtxU (CtxU Γ A2) A1) A0) v A ->
+  vcheck (CtxU (CtxU (CtxU Γ A0) A2) A1) (v_switch210_vars v) A
 
 with v_switch210_synthsafe
-  (Γ:ctx) (α2 : vtype) (α1:vtype) (α0:vtype) (v:val) (A:vtype)
+  (Γ:ctx) (A2 : vtype) (A1:vtype) (A0:vtype) (v:val) (A:vtype)
   {struct v}:
-  vsynth (CtxU (CtxU (CtxU Γ α2) α1) α0) v A ->
-  vsynth (CtxU (CtxU (CtxU Γ α0) α2) α1) (v_switch210_vars v) A
+  vsynth (CtxU (CtxU (CtxU Γ A2) A1) A0) v A ->
+  vsynth (CtxU (CtxU (CtxU Γ A0) A2) A1) (v_switch210_vars v) A
 
 with c_switch210_checksafe 
-  (Γ:ctx) (α2 : vtype) (α1:vtype) (α0:vtype) (c:comp) (C:ctype)
+  (Γ:ctx) (A2 : vtype) (A1:vtype) (A0:vtype) (c:comp) (C:ctype)
   {struct c}:
-  ccheck (CtxU (CtxU (CtxU Γ α2) α1) α0) c C -> 
-  ccheck (CtxU (CtxU (CtxU Γ α0) α2) α1) (c_switch210_vars c) C
+  ccheck (CtxU (CtxU (CtxU Γ A2) A1) A0) c C -> 
+  ccheck (CtxU (CtxU (CtxU Γ A0) A2) A1) (c_switch210_vars c) C
 
 with c_switch210_synthsafe 
-  (Γ:ctx) (α2 : vtype) (α1:vtype) (α0:vtype) (c:comp) (C:ctype)
+  (Γ:ctx) (A2 : vtype) (A1:vtype) (A0:vtype) (c:comp) (C:ctype)
   {struct c}:
-  csynth (CtxU (CtxU (CtxU Γ α2) α1) α0) c C -> 
-  csynth (CtxU (CtxU (CtxU Γ α0) α2) α1) (c_switch210_vars c) C
+  csynth (CtxU (CtxU (CtxU Γ A2) A1) A0) c C -> 
+  csynth (CtxU (CtxU (CtxU Γ A0) A2) A1) (c_switch210_vars c) C
 
 with h_switch210_checksafe
-  (Γ:ctx) (α2 : vtype) (α1:vtype) (α0:vtype) (h:hcases) (Σ:sig) (D:ctype)
+  (Γ:ctx) (A2 : vtype) (A1:vtype) (A0:vtype) (h:hcases) (Σ:sig) (D:ctype)
   {struct h}:
-  hcheck (CtxU (CtxU (CtxU Γ α2) α1) α0) h Σ D ->
-  hcheck (CtxU (CtxU (CtxU Γ α0) α2) α1) (h_switch210_vars h) Σ D.
+  hcheck (CtxU (CtxU (CtxU Γ A2) A1) A0) h Σ D ->
+  hcheck (CtxU (CtxU (CtxU Γ A0) A2) A1) (h_switch210_vars h) Σ D.
 Proof.
-all: intro orig; remember (CtxU (CtxU (CtxU Γ α2) α1) α0) as Γ'.
-all: remember (CtxU (CtxU (CtxU Γ α2) α0) α1) as Γ''.
-all: remember (CtxU (CtxU (CtxU Γ α0) α2) α1) as Γ'''.
-all: assert (get_vtype_i Γ' 0 = Some α0) as p_0.
+all: intro orig; remember (CtxU (CtxU (CtxU Γ A2) A1) A0) as Γ'.
+all: remember (CtxU (CtxU (CtxU Γ A2) A0) A1) as Γ''.
+all: remember (CtxU (CtxU (CtxU Γ A0) A2) A1) as Γ'''.
+all: assert (get_vtype_i Γ' 0 = Some A0) as p_0.
 all: try (rewrite HeqΓ'; simpl; f_equal).
-all: assert (get_vtype_i Γ' 1 = Some α1) as p_1.
+all: assert (get_vtype_i Γ' 1 = Some A1) as p_1.
 all: try (rewrite HeqΓ'; simpl; f_equal).
-all: assert (get_vtype_i Γ'' 1 = Some α0) as p'_0.
+all: assert (get_vtype_i Γ'' 1 = Some A0) as p'_0.
 all: try (rewrite HeqΓ''; simpl; f_equal).
-all: assert (get_vtype_i Γ'' 2 = Some α2) as p'_2.
+all: assert (get_vtype_i Γ'' 2 = Some A2) as p'_2.
 all: try (rewrite HeqΓ''; simpl; f_equal).
-all: assert (ctx_switch_vars Γ' 1 0 α1 α0 p_1 p_0 = Γ'').
+all: assert (ctx_switch_vars Γ' 1 0 A1 A0 p_1 p_0 = Γ'').
 all: try (unfold ctx_switch_vars; rewrite HeqΓ'; rewrite HeqΓ''; simpl; f_equal).
-all: assert (ctx_switch_vars Γ'' 2 1 α2 α0 p'_2 p'_0 = Γ''').
+all: assert (ctx_switch_vars Γ'' 2 1 A2 A0 p'_2 p'_0 = Γ''').
 all: try (unfold ctx_switch_vars; rewrite HeqΓ''; rewrite HeqΓ'''; simpl; f_equal).
 all: rewrite <-H0.
 + apply v_switch_checksafe. rewrite <-H.
